work on intLangTheory, up to Cevaluate_Clocs
also, add "closure_extra_data" to the semantics, to track information
associated with labels that isn't necessary for the implementation but
is useful for writing invariants. this is analogous to the "d" argument
previously, but now it's included in the code env (so fewer arguments to
deal with).

compiler/correctness/intLangScript.sml
@@ -22,7 +22,7 @@ rw[Once Cevaluate_cases] >> PROVE_TAC[])
 val Cevaluate_fun = store_thm(
 "Cevaluate_fun",
 ``∀c s env b res. Cevaluate c s env (CFun b) res =
-  (∀l. (b = INR l) ⇒ l ∈ FDOM c) ∧
+  (∀l. (b = INR l) ⇒ l ∈ FDOM c ∧ ((c ' l).nz = 1) ∧ ((c ' l).ez = LENGTH env)) ∧
   (res = (s, Rval (CRecClos env [b] 0)))``,
 rw[Once Cevaluate_cases] >> metis_tac[])
 
@@ -317,96 +317,13 @@ val Cevaluate_list_LENGTH = store_thm("Cevaluate_list_LENGTH",
 
 val FINITE_free_vars = store_thm(
 "FINITE_free_vars",
-``(∀c t. FINITE (free_vars c t)) ∧ (∀c b. FINITE (cbod_fvs c b))``,
+``(∀t. FINITE (free_vars t)) ∧ (∀b. FINITE (cbod_fvs b))``,
 ho_match_mp_tac free_vars_ind >>
 rw[free_vars_def] >>
-TRY (Cases_on `FLOOKUP c l` >> rw[] >> NO_TAC) >>
 rw[FOLDL_UNION_BIGUNION] >>
 TRY (match_mp_tac IMAGE_FINITE >> match_mp_tac FINITE_DIFF) >>
 metis_tac[])
 val _ = export_rewrites["FINITE_free_vars"]
-
-val free_vars_DOMSUB_SUBSET = store_thm("free_vars_DOMSUB_SUBSET",
-  ``(∀c e l. free_vars (c \\ l) e ⊆ free_vars c e) ∧
-    (∀c b l. cbod_fvs (c \\ l) b ⊆ cbod_fvs c b)``,
-  ho_match_mp_tac free_vars_ind >>
-  rw[FOLDL_UNION_BIGUNION,FOLDL_UNION_BIGUNION_paired] >>
-  fsrw_tac[DNF_ss][SUBSET_DEF] >>
-  fsrw_tac[DNF_ss][pairTheory.FORALL_PROD,pairTheory.EXISTS_PROD] >>
-  TRY (PROVE_TAC[]) >>
-  fsrw_tac[DNF_ss][FLOOKUP_DEF] >> rw[] >>
-  fsrw_tac[][DOMSUB_FAPPLY_THM] >>
-  first_x_assum match_mp_tac >>
-  metis_tac[DOMSUB_COMMUTES])
-
-val free_vars_DOMSUB = store_thm("free_vars_DOMSUB",
-  ``(∀c e l. (l ∈ FDOM c) ⇒ (free_vars c e ⊆ free_vars (c \\ l) e)) ∧
-    (∀c b l. (l ∈ FDOM c) ⇒ (cbod_fvs c b ⊆ cbod_fvs (c \\ l) b ∪ cbod_fvs (c \\ l) (INL ((c ' l).az,(c ' l).body))))``,
-  ho_match_mp_tac free_vars_ind >>
-  rw[FOLDL_UNION_BIGUNION] >>
-  fsrw_tac[DNF_ss][SUBSET_DEF] >>
-  TRY (metis_tac[]) >>
-  full_simp_tac(srw_ss()++QUANT_INST_ss[std_qp])[] >-
-
-  fs[FLOOKUP_DEF] >>
-  BasicProvers.CASE_TAC >>
-  BasicProvers.CASE_TAC >> fs[] >>
-  simp[DOMSUB_FAPPLY_THM] >>
-  metis_tac[DOMSUB_COMMUTES]
-  free_vars_def
-
-  strip_tac >- rw[] >>
-  strip_tac >- rw[] >>
-  strip_tac >- (
-    rw[] >> fsrw_tac[DNF_ss][SUBSET_DEF] >>
-    metis_tac[] ) >>
-  strip_tac >- rw[] >>
-  strip_tac >- rw[] >>
-  strip_tac >- rw[] >>
-  strip_tac >- (
-    rw[] >> fsrw_tac[DNF_ss][SUBSET_DEF] >>
-    simp_tac(srw_ss()++QUANT_INST_ss[std_qp])[] >-
-      metis_tac[] >>
-    rw[] >> res_tac >- metis_tac[] >>
-
-    fsrw_tac[ARITH_ss][ADD1] >>
-    TRY(metis_tac[])>>
-    rw[] >> res_tac >>
-    simp[]
-  strip_tac >- rw[] >>
-  strip_tac >- rw[] >>
-  strip_tac >- ...
-  strip_tac >- rw[] >>
-  strip_tac >- rw[] >>
-  strip_tac >- (
-    rw[] >> fsrw_tac[DNF_ss][SUBSET_DEF] >>
-    simp_tac(srw_ss()++QUANT_INST_ss[std_qp])[] >-
-      >- metis_tac[] >>
-    free_vars_def
-
-    rw[] >>
-  rw[FOLDL_UNION_BIGUNION,FOLDL_UNION_BIGUNION_paired] >>
-  fsrw_tac[DNF_ss][SUBSET_DEF] >>
-  fsrw_tac[DNF_ss][pairTheory.FORALL_PROD,pairTheory.EXISTS_PROD] >>
-  rw[] >> fsrw_tac[ARITH_ss][PRE_SUB1] >>
-  TRY (metis_tac[]) >>
-  spose_not_then strip_assume_tac >> fsrw_tac[ARITH_ss][] >>
-  BasicProvers.EVERY_CASE_TAC >>
-  fsrw_tac[DNF_ss][FLOOKUP_DEF] >> rw[] >>
-  fsrw_tac[][DOMSUB_FAPPLY_THM] >>
-  PROVE_TAC[DOMSUB_COMMUTES,free_vars_DOMSUB_SUBSET,SUBSET_DEF])
-
-val free_vars_SUBMAP = store_thm("free_vars_SUBMAP",
-  ``(∀c1 e c2. c1 ⊑ c2 ⇒ free_vars c1 e ⊆ free_vars c2 e) ∧
-    (∀c1 b c2. c1 ⊑ c2 ⇒ cbod_fvs c1 b ⊆ cbod_fvs c2 b)``,
-  ho_match_mp_tac free_vars_ind >>
-  rw[FOLDL_UNION_BIGUNION,FOLDL_UNION_BIGUNION_paired] >>
-  fsrw_tac[DNF_ss][SUBSET_DEF] >>
-  fsrw_tac[DNF_ss][SUBMAP_DEF] >>
-  fsrw_tac[DNF_ss][pairTheory.EXISTS_PROD,pairTheory.FORALL_PROD] >>
-  fsrw_tac[DNF_ss][FLOOKUP_DEF] >> rw[] >>
-  fsrw_tac[DNF_ss][DOMSUB_FAPPLY_THM] >>
-  metis_tac[])
 
 val find_index_ALL_DISTINCT_EL = store_thm(
 "find_index_ALL_DISTINCT_EL",
@@ -424,66 +341,9 @@ Induct >> rw[find_index_def] >>
 res_tac >>
 srw_tac[ARITH_ss][arithmeticTheory.ADD1])
 
-val fmap_rel_extend_rec_env_same = store_thm(
-"fmap_rel_extend_rec_env_same",
-``fmap_rel R env1 env2 ∧ LIST_REL R vs1 vs2 ∧ (LENGTH ns = LENGTH vs1) ∧
-  (∀b. MEM b rs ⇒ R (CRecClos cenv1 rs defs b) (CRecClos cenv2 rs defs b))
-  ⇒ fmap_rel R
-      (extend_rec_env cenv1 env1 rs defs ns vs1)
-      (extend_rec_env cenv2 env2 rs defs ns vs2)``,
-rw[extend_rec_env_def,FOLDL_FUPDATE_LIST,FOLDL2_FUPDATE_LIST,LIST_REL_EL_EQN] >>
-rw[MAP2_MAP,FST_pair,SND_pair,MAP_ZIP] >>
-match_mp_tac fmap_rel_FUPDATE_LIST_same >>
-rw[MAP_ZIP,LENGTH_ZIP,LIST_REL_EL_EQN] >>
-match_mp_tac fmap_rel_FUPDATE_LIST_same >>
-rw[MAP_ZIP,LENGTH_ZIP,LIST_REL_EL_EQN,EL_MAP,MAP_MAP_o,combinTheory.o_DEF] >>
-fsrw_tac[DNF_ss][MEM_EL])
-
-val FDOM_extend_rec_env = store_thm(
-"FDOM_extend_rec_env",
-``(LENGTH ns = LENGTH vs) ⇒ (FDOM (extend_rec_env cenv' env' ns' defs ns vs) = FDOM env' ∪ (set ns') ∪ (set ns))``,
-rw[extend_rec_env_def,FOLDL_FUPDATE_LIST,FOLDL2_FUPDATE_LIST,FDOM_FUPDATE_LIST] >>
-rw[MAP2_MAP,FST_pair,SND_pair,MAP_ZIP,MAP_MAP_o,combinTheory.o_DEF])
-val _ = export_rewrites["FDOM_extend_rec_env"]
-
-val extend_rec_env_FUNION = store_thm(
-"extend_rec_env_FUNION",
-``(LENGTH n = LENGTH v) ⇒
-  (extend_rec_env env f ns defs n v = extend_rec_env env FEMPTY ns defs n v ⊌ f)``,
-rw[extend_rec_env_def,FOLDL2_FUPDATE_LIST,FOLDL_FUPDATE_LIST] >>
-rw[MAP2_MAP,MAP_ZIP,FST_pair,SND_pair] >>
-fs[GSYM fmap_EQ_THM] >>
-conj_tac >- (
-  rw[FDOM_FUPDATE_LIST,MAP_ZIP,MAP2_MAP,FST_pair,SND_pair] >>
-  PROVE_TAC[UNION_COMM,UNION_ASSOC] ) >>
-qx_gen_tac `x` >>
-strip_tac >>
-Cases_on `MEM x n` >- (
-  Q.PAT_ABBREV_TAC `(f1 : string |-> Cv) = FEMPTY |++ MAP zz ns` >>
-  `x ∈ FDOM (f1 |++ ZIP (n,v))` by (
-    rw[FDOM_FUPDATE_LIST,MAP_ZIP] ) >>
-  rw[Once FUNION_DEF,SimpRHS] >>
-  match_mp_tac FUPDATE_SAME_LIST_APPLY >>
-  rw[MAP_ZIP] ) >>
-ho_match_mp_tac FUPDATE_LIST_APPLY_NOT_MEM_matchable >>
-fs[MAP_ZIP] >>
-Cases_on `MEM x ns` >- (
-  Q.PAT_ABBREV_TAC `(f1 : string |-> Cv) = FEMPTY |++ MAP zz ns` >>
-  `x ∈ FDOM (f1 |++ ZIP (n,v))` by (
-    rw[FDOM_FUPDATE_LIST,MAP_ZIP,Abbr`f1`,MAP_MAP_o,MEM_MAP] ) >>
-  rw[Once FUNION_DEF] >>
-  match_mp_tac FUPDATE_LIST_APPLY_NOT_MEM_matchable >>
-  rw[MAP_ZIP,Abbr`f1`] >>
-  match_mp_tac FUPDATE_SAME_LIST_APPLY >>
-  srw_tac[DNF_ss][MEM_MAP,MAP_MAP_o] ) >>
-rw[FUNION_DEF,FDOM_FUPDATE_LIST,MAP_ZIP,MAP_MAP_o,MEM_MAP] >>
-match_mp_tac EQ_SYM >>
-match_mp_tac FUPDATE_LIST_APPLY_NOT_MEM_matchable >>
-srw_tac[DNF_ss][MAP_MAP_o,MEM_MAP])
-
 val Cevaluate_store_SUBSET = store_thm("Cevaluate_store_SUBSET",
-  ``(∀c d s env exp res. Cevaluate c d s env exp res ⇒ FDOM s ⊆ FDOM (FST res)) ∧
-    (∀c d s env exps res. Cevaluate_list c d s env exps res ⇒ FDOM s ⊆ FDOM (FST res))``,
+  ``(∀c s env exp res. Cevaluate c s env exp res ⇒ FDOM s ⊆ FDOM (FST res)) ∧
+    (∀c s env exps res. Cevaluate_list c s env exps res ⇒ FDOM s ⊆ FDOM (FST res))``,
   ho_match_mp_tac Cevaluate_ind >> rw[] >>
   TRY (PROVE_TAC [SUBSET_TRANS]) >- (
     Cases_on`uop`>>rw[]>>rw[] >>
@@ -495,21 +355,12 @@ val Cevaluate_store_SUBSET = store_thm("Cevaluate_store_SUBSET",
 val all_Clocs_def = tDefine "all_Clocs"`
   (all_Clocs (CLitv _) = {}) ∧
   (all_Clocs (CConv _ vs) = BIGUNION (IMAGE all_Clocs (set vs))) ∧
-  (all_Clocs (CRecClos env _ _ _) = BIGUNION (IMAGE all_Clocs (FRANGE env))) ∧
+  (all_Clocs (CRecClos env _ _) = BIGUNION (IMAGE all_Clocs (set env))) ∧
   (all_Clocs (CLoc n) = {n})`
   (WF_REL_TAC`measure Cv_size` >>
-   srw_tac[ARITH_ss][fmap_size_def,FRANGE_DEF,Cvs_size_thm] >>
+   srw_tac[ARITH_ss][Cv1_size_thm] >>
    Q.ISPEC_THEN`Cv_size`imp_res_tac SUM_MAP_MEM_bound >>
-   fsrw_tac[ARITH_ss][] >>
-   qmatch_abbrev_tac `(q:num) < a + (y + (w + (z + 1)))` >>
-   qsuff_tac `q ≤ a` >- fsrw_tac[ARITH_ss][] >>
-   unabbrev_all_tac >>
-   qmatch_abbrev_tac `y <= SIGMA f (FDOM env)` >>
-   match_mp_tac LESS_EQ_TRANS >>
-   qexists_tac `f x` >>
-   conj_tac >- srw_tac[ARITH_ss][o_f_FAPPLY,Abbr`y`,Abbr`f`] >>
-   match_mp_tac SUM_IMAGE_IN_LE >>
-   rw[])
+   fsrw_tac[ARITH_ss][])
 val _ = export_rewrites["all_Clocs_def"]
 
 val CevalPrim2_Clocs = store_thm("CevaluatePrim2_Clocs",
@@ -518,15 +369,33 @@ val CevalPrim2_Clocs = store_thm("CevaluatePrim2_Clocs",
   TRY (Cases_on`l` >> fs[] >> Cases >> fs[] >> Cases_on `l` >> fs[] >> rw[] >> rw[]) >>
   Cases >> fs[] >> rw[] >> rw[])
 
+(* TODO: move *)
+val _ = export_rewrites["compileTermination.ceenv_def"]
+
+val good_cebind_def = Define`
+  (good_cebind ez nz (CERef n) = 0 < n ∧ n ≤ nz) ∧
+  (good_cebind ez nz (CEEnv n) = n < ez)`
+
+val all_Clocs_ceenv = store_thm("all_Clocs_ceenv",
+  ``∀env defs x. good_cebind (LENGTH env) (LENGTH defs) x ⇒
+  all_Clocs (ceenv env defs x) ⊆ BIGUNION (IMAGE all_Clocs (set env))``,
+  ntac 2 gen_tac >> Cases >> simp[SUBSET_DEF,MEM_EL,good_cebind_def] >>
+  srw_tac[DNF_ss][] >> metis_tac[])
+
+val good_cd_def = Define`
+  good_cd cd = EVERY (good_cebind cd.ez cd.nz) cd.cd.ceenv`
+
 val Cevaluate_Clocs = store_thm("Cevaluate_Clocs",
-  ``(∀c d s env exp res. Cevaluate c d s env exp res ⇒
-     BIGUNION (IMAGE all_Clocs (FRANGE env)) ⊆ FDOM s ∧
+  ``(∀c s env exp res. Cevaluate c s env exp res ⇒
+     (∀d. d ∈ FRANGE c ⇒ good_cd d) ∧
+     BIGUNION (IMAGE all_Clocs (set env)) ⊆ FDOM s ∧
      BIGUNION (IMAGE all_Clocs (FRANGE s)) ⊆ FDOM s
      ⇒
      BIGUNION (IMAGE all_Clocs (FRANGE (FST res))) ⊆ FDOM (FST res) ∧
      ∀v. (SND res = Rval v) ⇒ all_Clocs v ⊆ FDOM (FST res)) ∧
-    (∀c d s env exps res. Cevaluate_list c d s env exps res ⇒
-     BIGUNION (IMAGE all_Clocs (FRANGE env)) ⊆ FDOM s ∧
+    (∀c s env exps res. Cevaluate_list c s env exps res ⇒
+     (∀d. d ∈ FRANGE c ⇒ good_cd d) ∧
+     BIGUNION (IMAGE all_Clocs (set env)) ⊆ FDOM s ∧
      BIGUNION (IMAGE all_Clocs (FRANGE s)) ⊆ FDOM s
      ⇒
      BIGUNION (IMAGE all_Clocs (FRANGE (FST res))) ⊆ FDOM (FST res) ∧
@@ -544,7 +413,7 @@ val Cevaluate_Clocs = store_thm("Cevaluate_Clocs",
   strip_tac >- rw[] >>
   strip_tac >- (
     rw[] >>
-    fsrw_tac[DNF_ss][IN_FRANGE,SUBSET_DEF] >>
+    fsrw_tac[DNF_ss][SUBSET_DEF,MEM_EL] >>
     PROVE_TAC[] ) >>
   strip_tac >- rw[] >>
   strip_tac >- srw_tac[ETA_ss][] >>
@@ -567,39 +436,27 @@ val Cevaluate_Clocs = store_thm("Cevaluate_Clocs",
     rpt gen_tac >> ntac 2 strip_tac >>
     fs[] >> rfs[] >>
     first_x_assum match_mp_tac >>
-    rfs[FOLDL_FUPDATE_LIST] >>
-    fsrw_tac[DNF_ss][SUBSET_DEF] >>
-    map_every qx_gen_tac [`x`,`y`] >>
-    strip_tac >>
-    qpat_assum `x ∈ Y` mp_tac >>
-    pop_assum mp_tac >>
-    qid_spec_tac`y` >>
-    ho_match_mp_tac IN_FRANGE_FUPDATE_LIST_suff >>
-    fs[MAP_ZIP,AND_IMP_INTRO] >>
-    conj_tac >- PROVE_TAC[] >>
-    fsrw_tac[DNF_ss][MEM_MAP,FORALL_PROD] >>
+    fsrw_tac[DNF_ss][SUBSET_DEF,MEM_GENLIST] >>
     PROVE_TAC[] ) >>
   strip_tac >- srw_tac[ETA_ss][] >>
   strip_tac >- (
     rpt gen_tac >> ntac 2 strip_tac >>
     fs[] >> rfs[] >>
     first_x_assum match_mp_tac >>
-    simp[extend_rec_env_def,FOLDL2_FUPDATE_LIST,FOLDL_FUPDATE_LIST,MAP2_MAP,FST_pair,SND_pair,MAP_ZIP] >>
-    imp_res_tac Cevaluate_store_SUBSET >> fs[] >>
-    fsrw_tac[ETA_ss][] >>
-    reverse conj_tac >- PROVE_TAC[SUBSET_TRANS] >>
     fsrw_tac[DNF_ss][SUBSET_DEF] >>
-    map_every qx_gen_tac [`x`,`y`] >>
-    strip_tac >>
-    qpat_assum `x ∈ Y` mp_tac >>
-    pop_assum mp_tac >>
-    qid_spec_tac`y` >>
-    ho_match_mp_tac IN_FRANGE_FUPDATE_LIST_suff >>
-    simp[MAP_ZIP] >>
-    reverse conj_tac >- PROVE_TAC[SUBSET_TRANS] >>
-    ho_match_mp_tac IN_FRANGE_FUPDATE_LIST_suff >>
-    fsrw_tac[DNF_ss][MAP_MAP_o,combinTheory.o_DEF,MEM_MAP,EXISTS_PROD] >>
-    PROVE_TAC[] ) >>
+    Cases_on`cb`>>fs[LET_THM] >- (
+      PairCases_on`x`>>fs[]>>
+      fsrw_tac[DNF_ss][MEM_GENLIST]>>
+      imp_res_tac Cevaluate_store_SUBSET >>
+      fsrw_tac[DNF_ss][SUBSET_DEF] >>
+      metis_tac[] ) >>
+    fsrw_tac[DNF_ss][MEM_MAP,IN_FRANGE] >>
+    qmatch_assum_rename_tac`n < (c ' l).nz`[] >>
+    `good_cd (c ' l)` by metis_tac[] >>
+    fs[good_cd_def,EVERY_MEM] >>
+    imp_res_tac Cevaluate_store_SUBSET >>
+    fsrw_tac[DNF_ss][SUBSET_DEF] >>
+    metis_tac[SIMP_RULE(srw_ss()++DNF_ss)[SUBSET_DEF]all_Clocs_ceenv] ) >>
   strip_tac >- (
     rw[] >> fs[] >> rfs[] >>
     first_x_assum match_mp_tac >>
@@ -625,7 +482,7 @@ val Cevaluate_Clocs = store_thm("Cevaluate_Clocs",
     rw[] >> imp_res_tac CevalPrim2_Clocs >> rw[] ) >>
   strip_tac >- rw[] >>
   strip_tac >- (
-    ntac 7 gen_tac >>
+    ntac 6 gen_tac >>
     Cases >> fs[] >>
     gen_tac >> ntac 2 strip_tac >>
     fs[] >>
